src/lowparse/LowParse.Low.Int.fsti
@@ -2,6 +2,13 @@ module LowParse.Low.Int
 include LowParse.Spec.Int
 include LowParse.Low.Combinators
 
+module U16 = FStar.UInt16
+module U32 = FStar.UInt32
+module HST = FStar.HyperStack.ST
+module HS = FStar.HyperStack
+module B = LowStar.Buffer
+module M = LowStar.Modifies
+
 inline_for_extraction
 val parse32_u8: parser32 parse_u8
 
@@ -34,3 +41,27 @@ let validate_nochk32_u16 : validator_nochk32 parse_u16 =
 inline_for_extraction
 let validate_nochk32_u32 : validator_nochk32 parse_u32 =
   validate_nochk32_constant_size parse_u32 4ul ()
+
+val serialize32_u16
+  (b: buffer8)
+  (lo: U32.t)
+  (v: U16.t)
+: HST.Stack unit
+  (requires (fun h -> B.live h b /\ U32.v lo + 2 <= B.length b))
+  (ensures (fun h _ h' ->
+    M.modifies (M.loc_buffer (B.gsub b lo (2ul))) h h' /\
+    B.live h' b /\
+    exactly_contains_valid_data h' parse_u16 b lo v (U32.add lo 2ul)
+  ))
+
+val serialize32_u32
+  (b: buffer8)
+  (lo: U32.t)
+  (v: U32.t)
+: HST.Stack unit
+  (requires (fun h -> B.live h b /\ U32.v lo + 4 <= B.length b))
+  (ensures (fun h _ h' ->
+    M.modifies (M.loc_buffer (B.gsub b lo (4ul))) h h' /\
+    B.live h' b /\
+    exactly_contains_valid_data h' parse_u32 b lo v (U32.add lo 4ul)
+  ))
