src/lowparse/LowParseExample4.fst
@@ -1,0 +1,13 @@
+module LowParseExample4
+
+let parse_inner_kind = magic ()
+
+let parse_inner = magic ()
+
+let parse_inner_intro = magic ()
+
+let parse_t_kind = magic ()
+
+let parse_t = magic ()
+
+let parse_t_intro = magic ()
