src/lowparse/LowParseExample4.fsti
@@ -1,0 +1,80 @@
+module LowParseExample4
+
+module LPC = LowParse.Spec.Combinators
+module LPI = LowParse.Low.Int
+module LP = LowParse.Low.Base
+
+module U32 = FStar.UInt32
+module U16 = FStar.UInt16
+module HS = FStar.HyperStack
+module HST = FStar.HyperStack.ST
+module B = LowStar.Buffer
+
+noeq
+type inner = {
+  left: U16.t;
+  right: U16.t;
+}
+
+noeq
+type t = {
+  inner: inner;
+  last: U32.t;
+}
+
+val parse_inner_kind: (k: LP.parser_kind { k.LP.parser_kind_subkind == Some LP.ParserStrong})
+
+val parse_inner: LP.parser parse_inner_kind inner
+
+val parse_inner_intro
+  (h: HS.mem)
+  (b: LP.buffer8)
+  (lo: U32.t)
+  (x: U16.t * U16.t)
+  (hi: U32.t)
+: Lemma
+  (requires (
+    LP.exactly_contains_valid_data h (LPI.parse_u16 `LPC.nondep_then` LPI.parse_u16) b lo x hi
+  ))
+  (ensures (
+    let (l, r) = x in
+    LP.exactly_contains_valid_data h parse_inner b lo ({ left = l; right = r; }) hi
+  ))
+  [SMTPat (LP.exactly_contains_valid_data h (LPI.parse_u16 `LPC.nondep_then` LPI.parse_u16) b lo x hi)]
+
+val parse_t_kind : (k: LP.parser_kind { k.LP.parser_kind_subkind == Some LP.ParserStrong})
+
+val parse_t : LP.parser parse_t_kind t
+
+val parse_t_intro
+  (h: HS.mem)
+  (b: LP.buffer8)
+  (lo: U32.t)
+  (x: inner * U32.t)
+  (hi: U32.t)
+: Lemma
+  (requires (
+    LP.exactly_contains_valid_data h (parse_inner `LPC.nondep_then` LPI.parse_u32) b lo x hi
+  ))
+  (ensures (
+    let (l, r) = x in
+    LP.exactly_contains_valid_data h parse_t b lo ({ inner = l; last = r; }) hi
+  ))
+  [SMTPat (LP.exactly_contains_valid_data h (parse_inner `LPC.nondep_then` LPI.parse_u32) b lo x hi)]
+
+#set-options "--z3rlimit 32"
+
+let main: Int32.t -> FStar.Buffer.buffer (FStar.Buffer.buffer C.char) ->
+   HST.Stack C.exit_code (fun _ -> true) (fun _ _ _ -> true)
+=
+  fun _ _ ->
+  HST.push_frame ();
+  let b : LP.buffer8 = B.alloca 0uy 8ul in
+//  assert (B.len b == 8ul);
+  LPI.serialize32_u16 b 0ul 18us;
+  LPI.serialize32_u16 b 2ul 42us;
+  LPI.serialize32_u32 b 4ul 1729ul;
+  let h = HST.get () in
+  assert (LP.exactly_contains_valid_data h parse_t b 0ul ({ inner = ({ left = 18us; right = 42us; }); last = 1729ul;}) 8ul);
+  HST.pop_frame ();
+  C.EXIT_SUCCESS
